lakefile.lean
@@ -4,11 +4,14 @@ open Lake DSL
 package «spacetalk» where
   -- add any package configuration options here
 
-require batteries from
-  git "https://github.com/leanprover-community/batteries" @ "main"
+-- require batteries from
+--   git "https://github.com/leanprover-community/batteries" @ "main"
 
-require mathlib from git
-  "https://github.com/leanprover-community/mathlib4.git"
+-- require mathlib from
+--   git "https://github.com/leanprover-community/mathlib4.git"
+
+require smt from
+  git "https://github.com/ufmg-smite/lean-smt.git" @ "main"
 
 @[default_target]
 lean_lib «Spacetalk» where
